rustfrontend/InitDomain.v
@@ -447,6 +447,12 @@ Definition is_full (universe: PathsMap.t) (p: place) : bool :=
     let w := PathsMap.get (local_of_place p) universe in
     is_full_internal w p.
 
+Lemma is_full_same: forall w1 w2 p,
+    PathsMap.eq w1 w2 ->
+    is_full w1 p = is_full w2 p.
+Admitted.
+
+
 Record split_drop_place_spec (universe: Paths.t) (r: place) (drops: list (place * bool)) : Prop :=
   { split_sound: forall p, In p (map fst drops) -> Paths.In p universe /\ is_prefix r p = true;
     split_complete: forall p, Paths.In p universe -> is_prefix r p = true -> In p (map fst drops);
